library/data/vector.lean
@@ -92,6 +92,9 @@ end accum
 protected lemma eq {n : ℕ} : ∀ (a1 a2 : vector α n), to_list a1 = to_list a2 → a1 = a2
 | ⟨x, h1⟩ ⟨.x, h2⟩ rfl := rfl
 
+@[simp] lemma to_list_mk (v : list α) (P : list.length v = n) : to_list (subtype.mk v P) = v :=
+rfl
+
 @[simp] lemma to_list_nil : to_list [] = @list.nil α :=
 rfl
 
